more renamings

otbn_model/code/vale.dfy
@@ -41,12 +41,12 @@ module vt_vale {
 
     function va_get_reg32_t(r : reg32_t, s: va_state): uint32
     {
-        eval_reg32(s, r)
+        s.eval_reg32(r)
     }
 
     function va_get_reg256_t(r :reg256_t, s: va_state): uint256
     {
-        eval_reg256(s, r)
+        s.eval_reg256(r)
     }
 
     function va_get_fgroups(s: va_state): fgroups_t
@@ -143,7 +143,7 @@ module vt_vale {
 
     function va_eval_reg32(s: va_state, r : reg32_t):uint32
     {
-        s.gprs[r.index]
+        s.eval_reg32(r)
     }
 
     function va_update_operand_reg32(r: reg32_t, sM: va_state, sK: va_state): va_state
@@ -175,7 +175,7 @@ module vt_vale {
     function va_eval_reg256(s: va_state, r :reg256_t):uint256
         requires va_is_src_reg256(r, s);
     {
-        eval_reg256(s, r)
+        s.eval_reg256(r)
     }
 
     function va_update_operand_reg256(r :reg256_t, sM: va_state, sK: va_state): va_state
@@ -200,14 +200,14 @@ module vt_vale {
         && s0.ok == s1.ok
     }
 
-    predicate{:opaque} evalCodeOpaque(c:code, s0:state, sN:state)
+    predicate{:opaque} eval_code_opaque(c:code, s0:state, sN:state)
     {
-        evalCode(c, s0, sN)
+        eval_code(c, s0, sN)
     }
 
-    predicate eval_code(c:code, s:state, r:state)
+    predicate eval_code_lax(c:code, s:state, r:state)
     {
-        s.ok ==> evalCodeOpaque(c, s, r)
+        s.ok ==> eval_code_opaque(c, s, r)
     }
 
     function method va_CNil():codes { CNil }
@@ -217,22 +217,22 @@ module vt_vale {
     predicate va_require(b0:codes, c1:code, s0: va_state, sN: va_state)
     {
         && cHeadIs(b0, c1)
-        && eval_code(Block(b0), s0, sN)
-        && BN_ValidState(s0)
+        && eval_code_lax(Block(b0), s0, sN)
+        && valid_state_opaque(s0)
     }
 
     // Weaker form of eval_code that we can actually ensure generically in instructions
     predicate eval_weak(c:code, s:state, r:state)
     {
-        s.ok && r.ok ==> evalCodeOpaque(c, s, r)
+        s.ok && r.ok ==> eval_code_opaque(c, s, r)
     }
 
     predicate va_ensure(b0:codes, b1:codes, s0: va_state, s1: va_state, sN: va_state)
     {
         && cTailIs(b0, b1)
         && eval_weak(b0.hd, s0, s1)
-        && eval_code(Block(b1), s1, sN)
-        && BN_ValidState(s1)
+        && eval_code_lax(Block(b1), s1, sN)
+        && valid_state_opaque(s1)
     }
 
     lemma va_ins_lemma(b0:code, s0: va_state)
@@ -255,12 +255,12 @@ module vt_vale {
     function method va_get_whileBody(c:code):code requires c.While? { c.whileBody }
 
     lemma lemma_FailurePreservedByBlock(block:codes, s:state, r:state)
-        requires evalBlock(block, s, r);
+        requires eval_block(block, s, r);
         ensures !s.ok ==> !r.ok;
         decreases block;
     {
         if !block.CNil? {
-            var r' :| evalCode(block.hd, s, r') && evalBlock(block.tl, r', r);
+            var r' :| eval_code(block.hd, s, r') && eval_block(block.tl, r', r);
             lemma_FailurePreservedByCode(block.hd, s, r');
             lemma_FailurePreservedByBlock(block.tl, r', r);
         }
@@ -268,7 +268,7 @@ module vt_vale {
 
 
     lemma lemma_FailurePreservedByCode(c:code, s:state, r:state)
-        requires evalCode(c, s, r);
+        requires eval_code(c, s, r);
         ensures !s.ok ==> !r.ok;
     {
         match c {
@@ -276,25 +276,25 @@ module vt_vale {
                 lemma_FailurePreservedByBlock(b, s, r);
             }
             case While(c, b) => {
-                var n :| evalWhile(b, n, s, r);
+                var n :| eval_while(b, n, s, r);
             }
             case Ins256(i) => {
-                var r' :| evalCode(c, s, r');
+                var r' :| eval_code(c, s, r');
             }
             case Ins32(i) => {
-                var r' :| evalCode(c, s, r');
+                var r' :| eval_code(c, s, r');
             }
         }
     }
 
     lemma block_state_validity(block:codes, s:state, r:state)
-        requires evalBlock(block, s, r);
+        requires eval_block(block, s, r);
         requires valid_state(s);
         decreases block, 0;
         ensures r.ok ==> valid_state(r);
     {
         if block.va_CCons? {
-            var r':state :| evalCode(block.hd, s, r') && evalBlock(block.tl, r', r);
+            var r':state :| eval_code(block.hd, s, r') && eval_block(block.tl, r', r);
             code_state_validity(block.hd, s, r');
             if r'.ok {
                 block_state_validity(block.tl, r', r);
@@ -304,21 +304,21 @@ module vt_vale {
         }
     }
 
-    lemma evalWhile_validity(w:whileCond, c:code, n:nat, s:state, r:state)
-        requires evalWhile(c, n, s, r);
+    lemma eval_while_validity(w:whileCond, c:code, n:nat, s:state, r:state)
+        requires eval_while(c, n, s, r);
         decreases c, 1, n;
         ensures valid_state(s) && r.ok ==> valid_state(r);
     {
         if valid_state(s) && r.ok && n > 0 {
-            var r' :| evalCode(c, s, r') && evalWhile(c, n - 1, r', r);
+            var r' :| eval_code(c, s, r') && eval_while(c, n - 1, r', r);
             code_state_validity(c, s, r');
-            evalWhile_validity(w, c, n - 1, r', r);
+            eval_while_validity(w, c, n - 1, r', r);
             assert valid_state(r);
         }
     }
 
     lemma code_state_validity(c:code, s:state, r:state)
-        requires evalCode(c, s, r);
+        requires eval_code(c, s, r);
         requires valid_state(s);
         decreases c, 0;
         ensures  r.ok ==> valid_state(r);
@@ -331,89 +331,89 @@ module vt_vale {
             } else if c.Block? {
                 block_state_validity(c.block, s, r);
             } else if c.While? {
-                var n:nat :| evalWhile(c.whileBody, n, s, r);
-                evalWhile_validity(c.whileCond, c.whileBody, n, s, r);
+                var n:nat :| eval_while(c.whileBody, n, s, r);
+                eval_while_validity(c.whileCond, c.whileBody, n, s, r);
                 assert valid_state(r);
             }
         } 
     }
 
     lemma va_lemma_empty(s: va_state, r: va_state) returns(r': va_state)
-        requires eval_code(Block(va_CNil()), s, r)
+        requires eval_code_lax(Block(va_CNil()), s, r)
         ensures  s.ok ==> r.ok
         ensures  r' == s
         ensures  s.ok ==> r == s
     {
-        reveal_evalCodeOpaque();
+        reveal_eval_code_opaque();
         r' := s;
     }
 
-    predicate {:opaque} BN_ValidState(s:state)
-        ensures BN_ValidState(s) ==> valid_state(s);
+    predicate {:opaque} valid_state_opaque(s:state)
+        ensures valid_state_opaque(s) ==> valid_state(s);
     {
         valid_state(s)
     }
 
     lemma va_lemma_block(b:codes, s0: va_state, r: va_state) returns(r1: va_state, c0:code, b1:codes)
         requires b.va_CCons?
-        requires eval_code(Block(b), s0, r)
+        requires eval_code_lax(Block(b), s0, r)
         ensures  b == va_CCons(c0, b1)
-        ensures  eval_code(c0, s0, r1)
-            ensures BN_ValidState(s0) && r1.ok ==> BN_ValidState(r1);
-        ensures  eval_code(Block(b1), r1, r)
+        ensures  eval_code_lax(c0, s0, r1)
+            ensures valid_state_opaque(s0) && r1.ok ==> valid_state_opaque(r1);
+        ensures  eval_code_lax(Block(b1), r1, r)
     {
-        reveal_evalCodeOpaque();
+        reveal_eval_code_opaque();
         c0 := b.hd;
         b1 := b.tl;
         if s0.ok {
-            assert evalBlock(b, s0, r);
-            var r':state :| evalCode(b.hd, s0, r') && evalBlock(b.tl, r', r);
+            assert eval_block(b, s0, r);
+            var r':state :| eval_code(b.hd, s0, r') && eval_block(b.tl, r', r);
             c0 := b.hd;
             b1 := b.tl;
             r1 := state(r'.gprs, r'.wdrs, r'.wmod, r'.wrnd, r'.wacc, r'.fgroups, r'.xmem, r'.wmem, r'.ok);
-            if BN_ValidState(s0) {
-                reveal_BN_ValidState();
+            if valid_state_opaque(s0) {
+                reveal_valid_state_opaque();
                 code_state_validity(c0, s0, r1);
             }
-            assert eval_code(c0, s0, r1);
+            assert eval_code_lax(c0, s0, r1);
         } else {
             // If s0 isn't okay, we can do whatever we want,
-            // so we ensure r1.ok is false, and hence eval_code(*, r1, *) is trivially true
+            // so we ensure r1.ok is false, and hence eval_code_lax(*, r1, *) is trivially true
             r1 := s0;
         }
     }
 
-    predicate {:opaque} evalWhileOpaque(w:whileCond, c:code, n:nat, s:state, r:state)
+    predicate {:opaque} eval_while_opaque(w:whileCond, c:code, n:nat, s:state, r:state)
     {
-        evalWhile(c, n, s, r)
+        eval_while(c, n, s, r)
     }
 
-    predicate evalWhileLax(w:whileCond, c:code, n:nat, s:state, r:state)
+    predicate eval_while_lax(w:whileCond, c:code, n:nat, s:state, r:state)
     {
-        s.ok ==> evalWhileOpaque(w, c, n, s, r)
+        s.ok ==> eval_while_opaque(w, c, n, s, r)
     }
 
     predicate va_whileInv(w:whileCond, c:code, n:int, r1: va_state, r2: va_state)
     {
-        n >= 0 && BN_ValidState(r1) && evalWhileLax(w, c, n, r1, r2)
+        n >= 0 && valid_state_opaque(r1) && eval_while_lax(w, c, n, r1, r2)
     }
 
     lemma va_lemma_while(w:whileCond, c:code, s: va_state, r: va_state) returns(n:nat, r': va_state)
         // requires va_is_src_reg32(w.r, s);
         // requires va_is_src_imm32(w.c, s);
-        requires BN_ValidState(s);
-        requires eval_code(While(w, c), s, r)
-        ensures  evalWhileLax(w, c, n, r', r)
+        requires valid_state_opaque(s);
+        requires eval_code_lax(While(w, c), s, r)
+        ensures  eval_while_lax(w, c, n, r', r)
         //ensures  r'.ok
         ensures s.ok ==> (n == eval_cond(s, w));
-        ensures  BN_ValidState(r');
+        ensures  valid_state_opaque(r');
         ensures r' == s
     {
-        reveal_evalCodeOpaque();
-        reveal_BN_ValidState();
-        reveal_evalWhileOpaque();
+        reveal_eval_code_opaque();
+        reveal_valid_state_opaque();
+        reveal_eval_while_opaque();
         if s.ok {
-            assert evalCode(While(w, c), s, r);
+            assert eval_code(While(w, c), s, r);
             n := eval_cond(s, w);
         } else {
             n := 0;
@@ -425,31 +425,31 @@ module vt_vale {
         // requires va_is_src_reg32(w.r, s) && ValidSourceRegister32(s, w.r);
         // requires va_is_src_imm32(w.c, s);
         requires n > 0
-        requires evalWhileLax(w, c, n, s, r)
-        ensures  BN_ValidState(s) ==> BN_ValidState(s');
-        ensures  evalWhileLax(w, c, n - 1, r', r)
-        ensures  eval_code(c, s', r');
-        // ensures  BN_ValidState(s) ==> if s.ok then BN_branchRelation(s, s', true) else s' == s;
-        ensures  if s.ok && BN_ValidState(s) then
+        requires eval_while_lax(w, c, n, s, r)
+        ensures  valid_state_opaque(s) ==> valid_state_opaque(s');
+        ensures  eval_while_lax(w, c, n - 1, r', r)
+        ensures  eval_code_lax(c, s', r');
+        // ensures  valid_state_opaque(s) ==> if s.ok then BN_branchRelation(s, s', true) else s' == s;
+        ensures  if s.ok && valid_state_opaque(s) then
                     && s'.ok
                     && s == s'
                     // && eval_cond(s, w) > 0
                 else
                     true; //!r.ok;
     {
-        reveal_evalCodeOpaque();
-        reveal_evalWhileOpaque();
-        reveal_BN_ValidState();
+        reveal_eval_code_opaque();
+        reveal_eval_while_opaque();
+        reveal_valid_state_opaque();
 
         if !s.ok {
             s' := s;
             r' := s;
             return;
         }
-        assert evalWhile(c, n, s, r); // TODO: Dafny reveal/opaque issue
+        assert eval_while(c, n, s, r); // TODO: Dafny reveal/opaque issue
 
-        if BN_ValidState(s) {
-            var r'':state :| evalCode(c, s, r'') && evalWhile( c, n - 1, r'', r);
+        if valid_state_opaque(s) {
+            var r'':state :| eval_code(c, s, r'') && eval_while( c, n - 1, r'', r);
             s' := s;
             r' := r'';
             code_state_validity(c, s', r'');
@@ -460,10 +460,10 @@ module vt_vale {
     }
 
     lemma va_lemma_whileFalse(w:whileCond, c:code, s: va_state, r: va_state) returns(r': va_state)
-        requires evalWhileLax(w, c, 0, s, r)
+        requires eval_while_lax(w, c, 0, s, r)
         ensures  if s.ok then
-                    (if BN_ValidState(s) then
-                        (r'.ok ==> BN_ValidState(r'))
+                    (if valid_state_opaque(s) then
+                        (r'.ok ==> valid_state_opaque(r'))
                     //  && BN_branchRelation(s, r', false)
                     //  && eval_cond(s, w) == 0
                     && s == r
@@ -474,9 +474,9 @@ module vt_vale {
                 else
                     r' == s; //!r.ok;
     {
-        reveal_evalCodeOpaque();
-        reveal_evalWhileOpaque();
-        reveal_BN_ValidState();
+        reveal_eval_code_opaque();
+        reveal_eval_while_opaque();
+        reveal_valid_state_opaque();
 
         if !s.ok {
             r' := s;
